theories/iris/rules/iris_rules_calls.v
@@ -186,7 +186,7 @@ Qed.
       eapply lfilled_to_val in Hcontr;[|eauto].
       inversion Hcontr.
       done. }
-    iIntros ([[ ? ?] ?] ns κ κs nt) "(Hσ1&Hσ2&Hσ3&Hσ4&Hσ5&Hσ6)".
+    iIntros ([[ ? ?] ?] ns κ κs nt) "(Hσ1&Hσ2&Hσ3&Hσ4&Hσ7&Hσ8&Hσ5&Hσ6)".
     iApply fupd_frame_l.
     iDestruct (ghost_map_lookup with "Hσ5 Hf") as %Hlook. simplify_map_eq.
     set (σ := (s0,l,i0)).
@@ -245,7 +245,7 @@ Qed.
       eapply lfilled_to_val in Hcontr;[|eauto].
       inversion Hcontr.
       done. }
-    iIntros ([[ ? ?] ?] ns κ κs nt) "(Hσ1&Hσ2&Hσ3&Hσ4&Hσ5&Hσ6)".
+    iIntros ([[ ? ?] ?] ns κ κs nt) "(Hσ1&Hσ2&Hσ3&Hσ4&Hσ7&Hσ8&Hσ5&Hσ6)".
     iApply fupd_frame_l.
     iDestruct (gen_heap_valid with "Hσ2 Ha") as %Hlook.
     iDestruct (gen_heap_valid with "Hσ1 Hcl") as %Hlook2.
@@ -322,7 +322,7 @@ Qed.
   Proof.
     iIntros (Htype Hc) "Ha Hcl Hf Hcont".
     iApply wp_lift_atomic_step;[auto|].
-    iIntros ([[ ? ?] ?] ns κ κs nt) "(Hσ1&Hσ2&Hσ3&Hσ4&Hσ5&Hσ6)".
+    iIntros ([[ ? ?] ?] ns κ κs nt) "(Hσ1&Hσ2&Hσ3&Hσ4&?&?&Hσ5&Hσ6)".
     iApply fupd_frame_l.
     iDestruct (gen_heap_valid with "Hσ2 Ha") as %Hlook.
     iDestruct (gen_heap_valid with "Hσ1 Hcl") as %Hlook2.
@@ -368,7 +368,7 @@ Qed.
   Proof.
     iIntros (Hc) "Hf Hcont".
     iApply wp_lift_atomic_step;[auto|].
-    iIntros ([[? ?] ?] ns κ κs nt) "(Hσ1&Hσ2&Hσ3&Hσ4&Hσ5&Hσ6)".
+    iIntros ([[? ?] ?] ns κ κs nt) "(Hσ1&Hσ2&Hσ3&Hσ4&?&?&Hσ5&Hσ6)".
     iApply fupd_frame_l.
     iDestruct (ghost_map_lookup with "Hσ5 Hf") as %Hf. simplify_map_eq.
     simplify_lookup.
@@ -405,7 +405,7 @@ Qed.
   Proof.
     iIntros (Hc) "Ha Hf Hcont".
     iApply wp_lift_atomic_step;[auto|].
-    iIntros ([[ ? ?] ?] ns κ κs nt) "(Hσ1&Hσ2&Hσ3&Hσ4&Hσ5&Hσ6)".
+    iIntros ([[ ? ?] ?] ns κ κs nt) "(Hσ1&Hσ2&Hσ3&Hσ4&?&?&Hσ5&Hσ6)".
     iApply fupd_frame_l.
     iDestruct (gen_heap_valid with "Hσ2 Ha") as %Hlook.
     iDestruct (ghost_map_lookup with "Hσ5 Hf") as %Hf. simplify_map_eq.
@@ -447,7 +447,7 @@ Qed.
   Proof.
     iIntros (Hc Hge) "#Ha Hf Hcont".
     iApply wp_lift_atomic_step;[auto|].
-    iIntros ([[ ? ?] ?] ns κ κs nt) "(Hσ1&Hσ2&Hσ3&Hσ4&Hσ5&Hσ6&Hσ7&Hσ8&Hσ9)".
+    iIntros ([[ ? ?] ?] ns κ κs nt) "(Hσ1&Hσ2&Hσ3&Hσ4&?&?&Hσ5&Hσ6&?&Hσ7&Hσ8&Hσ9)".
     iApply fupd_frame_l.
     iDestruct (gen_heap_valid with "Hσ7 Ha") as %Hlook.
     rewrite gmap_of_list_lookup Nat2N.id in Hlook.
