theories/iris/rules/iris_rules_resources.v
@@ -147,7 +147,7 @@ Proof.
   iApply wp_lift_atomic_step => //=.
   iIntros (σ ns κ κs nt) "Hσ !>".
   destruct σ as [[ws locs] inst].
-  iDestruct "Hσ" as "(? & ? & ? & ? & ? & Hl & ?)".
+  iDestruct "Hσ" as "(? & ? & ? & ? & ? & ? & Hl & ?)".
   iDestruct (ghost_map_lookup with "Hl Hli") as "%Hli".
   simplify_map_eq.
   rewrite - nth_error_lookup in Hlook.
@@ -175,7 +175,7 @@ Proof.
   iApply wp_lift_atomic_step => //=.
   iIntros (σ ns κ κs nt) "Hσ !>".
   destruct σ as [[ws locs] inst].
-  iDestruct "Hσ" as "(? & ? & ? & ? & ? & Hl & ?)".
+  iDestruct "Hσ" as "(? & ? & ? & ? & ? & ? & Hl & ?)".
   iDestruct (ghost_map_lookup with "Hl Hli") as "%Hli".
   simplify_map_eq.
   iSplit.
@@ -243,7 +243,7 @@ Proof.
   iApply wp_lift_atomic_step => //=.
   iIntros (σ ns κ κs nt) "Hσ !>".
   destruct σ as [[ws locs] winst].
-  iDestruct "Hσ" as "(? & ? & ? & ? & Hg & Hi & ? & ?)".
+  iDestruct "Hσ" as "(? & ? & ? & ? & ? & Hg & Hi & ? & ?)".
   iDestruct (gen_heap_valid with "Hg Hglob") as "%Hglob".
   iDestruct (ghost_map_lookup with "Hi Hinst") as "%Hli".
   simplify_map_eq.
@@ -282,7 +282,7 @@ Proof.
   iApply wp_lift_atomic_step => //=.
   iIntros (σ ns κ κs nt) "Hσ !>".
   destruct σ as [[ws locs] winst].
-  iDestruct "Hσ" as "(? & ? & ? & ? & Hg & Hi & ? & ?)".
+  iDestruct "Hσ" as "(? & ? & ? & ? & ? & Hg & Hi & ? & ?)".
   iDestruct (gen_heap_valid with "Hg Hglob") as "%Hglob".
   iDestruct (ghost_map_lookup with "Hi Hinst") as "%Hli".
   simplify_map_eq.
@@ -1792,7 +1792,7 @@ Proof.
   iApply wp_lift_atomic_step => //=.
   iIntros (σ ns κ κs nt) "Hσ !>".
   destruct σ as [[ws locs] winst].
-  iDestruct "Hσ" as "(? & ? & Hm & ? & ? & Hframe & Hγ)".
+  iDestruct "Hσ" as "(? & ? & Hm & ? & ? & ? & Hframe & Hγ)".
   iDestruct (ghost_map_lookup with "Hframe Hf0") as "%Hf0".
   rewrite lookup_insert in Hf0.
   inversion Hf0; subst; clear Hf0.
@@ -1865,7 +1865,7 @@ Proof.
   iApply wp_lift_atomic_step => //=.
   iIntros (σ ns κ κs nt) "Hσ !>".
   destruct σ as [[ws locs] winst].
-  iDestruct "Hσ" as "(? & ? & Hm & ? & ? & Hframe & Hγ)".
+  iDestruct "Hσ" as "(? & ? & Hm & ? & ? & ? & Hframe & Hγ)".
   iDestruct (ghost_map_lookup with "Hframe Hf0") as "%Hf0".
   rewrite lookup_insert in Hf0.
   inversion Hf0; subst; clear Hf0.
@@ -1916,7 +1916,7 @@ Proof.
   iApply wp_lift_atomic_step => //=.
   iIntros (σ ns κ κs nt) "Hσ !>".
   destruct σ as [[ ws locs] winst].
-  iDestruct "Hσ" as "(? & ? & Hm & ? & ? & Hframe & Hγ & ?)".
+  iDestruct "Hσ" as "(? & ? & Hm & ? & ? & ? & Hframe & Hγ & ?)".
   iDestruct (ghost_map_lookup with "Hframe Hf0") as "%Hf0".
   iAssert (⌜is_Some (s_mems ws !! n)⌝)%I as %[m Hm].
   { iDestruct (gen_heap_valid with "Hγ Hwms") as %HH.
@@ -1965,7 +1965,7 @@ Proof.
   iApply wp_lift_atomic_step => //=.
   iIntros (σ ns κ κs nt) "Hσ !>".
   destruct σ as [[ws locs] winst].
-  iDestruct "Hσ" as "(? & ? & Hm & ? & ? & Hframe & Hγ & ?)".
+  iDestruct "Hσ" as "(? & ? & Hm & ? & ? & ? & Hframe & Hγ & ?)".
   iDestruct (ghost_map_lookup with "Hframe Hf0") as "%Hf0".
   iAssert (⌜is_Some (s_mems ws !! n)⌝)%I as %[m Hm].
   { iDestruct (gen_heap_valid with "Hγ Hwms") as %HH.
@@ -2016,7 +2016,7 @@ Proof.
   iApply wp_lift_atomic_step => //=.
   iIntros (σ ns κ κs nt) "Hσ !>".
   destruct σ as [[ws locs] winst].
-  iDestruct "Hσ" as "(? & ? & Hm & ? & ? & Hframe & Hmemlength & ? & Hmemlimit & ?)".
+  iDestruct "Hσ" as "(? & ? & Hm & ? & ? & ? & Hframe & Hmemlength & ? & Hmemlimit & ?)".
   iDestruct (ghost_map_lookup with "Hframe Hf0") as "%Hf0".
   rewrite lookup_insert in Hf0.
   inversion Hf0; subst; clear Hf0.
@@ -2101,7 +2101,7 @@ Proof.
   iApply wp_lift_atomic_step => //=.
   iIntros (σ ns κ κs nt) "Hσ !>".
   destruct σ as [[ ws locs] winst].
-  iDestruct "Hσ" as "(? & ? & Hm & ? & ? & Hframe & Hmemlength & ? & Hmemlimit & ?)".
+  iDestruct "Hσ" as "(? & ? & Hm & ? & ? & ? & Hframe & Hmemlength & ? & Hmemlimit & ?)".
   iDestruct (ghost_map_lookup with "Hframe Hf0") as "%Hf0".
   rewrite lookup_insert in Hf0.
   inversion Hf0; subst; clear Hf0.
@@ -2168,7 +2168,7 @@ Proof.
   iApply wp_lift_atomic_step => //=.
   iIntros (σ ns κ κs nt) "Hσ !>".
   destruct σ as [[ws locs] winst].
-  iDestruct "Hσ" as "(? & ? & Hm & ? & ? & Hframe & Hγ & ?)".
+  iDestruct "Hσ" as "(? & ? & Hm & ? & ? & ? & Hframe & Hγ & ?)".
   iDestruct (ghost_map_lookup with "Hframe Hf0") as "%Hf0".
   iAssert (⌜is_Some (s_mems ws !! n)⌝)%I as %[m Hm].
   { iDestruct (gen_heap_valid with "Hγ Hwms") as %HH.
@@ -2216,7 +2216,7 @@ Proof.
   iApply wp_lift_atomic_step => //=.
   iIntros (σ ns κ κs nt) "Hσ !>".
   destruct σ as [[ ws locs] winst].
-  iDestruct "Hσ" as "(? & ? & Hm & ? & ? & Hframe & Hγ & ?)".
+  iDestruct "Hσ" as "(? & ? & Hm & ? & ? & ? & Hframe & Hγ & ?)".
   iDestruct (ghost_map_lookup with "Hframe Hf0") as "%Hf0".
   iAssert (⌜is_Some (s_mems ws !! n)⌝)%I as %[m Hm].
   { iDestruct (gen_heap_valid with "Hγ Hwms") as %HH.
@@ -2263,7 +2263,7 @@ Proof.
   iApply wp_lift_atomic_step => //=.
   iIntros (σ ns κ κs nt) "Hσ !>".
   destruct σ as [[ws locs] winst].
-  iDestruct "Hσ" as "(? & ? & Hm & ? & ? & Hframe & Hγ & ?)".
+  iDestruct "Hσ" as "(? & ? & Hm & ? & ? & ? & Hframe & Hγ & ?)".
   iDestruct (ghost_map_lookup with "Hframe Hf0") as "%Hframe".
   iDestruct (gen_heap_valid with "Hγ Hmemlength") as "%Hmemlength".
   rewrite lookup_insert in Hframe.
@@ -2546,7 +2546,7 @@ Proof.
   iApply wp_lift_atomic_step => //=.
   iIntros (σ ns κ κs nt) "Hσ !>".
   destruct σ as [[ws  locs ] winst].
-  iDestruct "Hσ" as "(? & ? & Hm & ? & ? & Hf & Hmemlength & ? & ? & Hmemlimit & ?)".
+  iDestruct "Hσ" as "(? & ? & Hm & ? & ? & ? & Hf & Hmemlength & ? & ? & Hmemlimit & ?)".
   iDestruct (ghost_map_lookup with "Hf Hframe") as "%Hframe".
   iDestruct (gen_heap_valid with "Hmemlength Hmlength") as "%Hmemlength".
   rewrite lookup_insert in Hframe.
